fixtures/TypeChecker.mli
@@ -796,11 +796,21 @@ val check_fn_root_shadow_provenance_summary : global_env -> fn_def -> bool
 
 val check_env_root_shadow_provenance_summary : global_env -> bool
 
+val direct_call_ready_expr_b : expr -> bool
+
+val check_fn_root_shadow_direct_call_provenance_summary :
+  global_env -> fn_def -> bool
+
+val check_env_root_shadow_direct_call_provenance_summary : global_env -> bool
+
 val check_env_preservation_ready : global_env -> bool
 
 val check_program_env_alpha_validated_root_shadow : global_env -> bool
 
 val check_program_env_alpha_validated_root_shadow_provenance_summary :
+  global_env -> bool
+
+val check_program_env_alpha_validated_root_shadow_direct_call_provenance_summary :
   global_env -> bool
 
 val check_program_env_alpha_validated_root_shadow_provenance :
